code/rocq/valid_state.v
@@ -62,7 +62,7 @@ Module valid_state (U:Unif).
 
   Fixpoint valid_state s :=
     match s with
-    | Goal _ _ | OK _ | KO | Bot | Top => true
+    | Goal _ _ | OK | KO | Bot | Top => true
     | Dead => false
     | Or A _ B => 
       if A == dead A then valid_state B
